src/Narcissus/Examples/NetworkStack/EthernetHeader.v
@@ -77,93 +77,193 @@ Section EthernetPacketDecoder.
 
   Definition ethernet_Header_OK (e : EthernetHeader) := True.
 
-  Definition v1042_test : DecodeM (bool * ByteString) ByteString :=
-    fun t env =>
-    `(w, t', env') <- decode_word t env;
-      if (wlt_dec w (natToWord 16 1501) : bool) then
-         Some (true, t', env') else Some (false, t', env').
-
-  Lemma derive_distinguishing_word SourcePred
-    : forall P P_inv,
-      cache_inv_Property P P_inv ->
-    CorrectDecoder ByteStringQueueMonoid
-                   SourcePred
+  Lemma derive_distinguishing_word v0 v1
+    : forall
+      P (P_OK : cache_inv_Property P (fun P => forall b cd, P cd -> P (addD cd b))),
+      CorrectRefinedDecoder ByteStringQueueMonoid
+       (fun s : EthernetHeader => (ethernet_Header_OK s /\ IsProj Destination v1 s) /\ IsProj Source v0 s)
     (constant True) (constant (constant True))
     (Either format_nat 16 ◦ constant packet_len ++
             format_word ◦ constant WO~0~1~0~1~0~1~0~1 ++
             format_word ◦ constant WO~0~1~0~1~0~1~0~1 ++
             format_word ◦ constant WO~1~1~0~0~0~0~0~0 ++
             format_word ◦ constant wzero 24 ++ format_enum EtherTypeCodes ◦ EthType ++ empty_Format
-     Or format_enum EtherTypeCodes ◦ EthType ++ empty_Format) v1042_test P
+            Or format_enum EtherTypeCodes ◦ EthType ++ empty_Format)
+    (format_unused_word 16)
+    (fun t env =>
+    `(w, t', env') <- decode_word t env;
+      if (wlt_dec w (natToWord 16 1501) : bool) then
+         Some (true, t', env') else Some (false, t', env')) P
     (fun (bs : bool) (env : CacheFormat) (t : ByteString * CacheFormat) =>
-     forall s : EthernetHeader,
+     forall (s : EthernetHeader) (t' : ByteString) (env' : CacheFormat),
      ((format_nat 16 ◦ constant packet_len ++
        format_word ◦ constant WO~0~1~0~1~0~1~0~1 ++
        format_word ◦ constant WO~0~1~0~1~0~1~0~1 ++
        format_word ◦ constant WO~1~1~0~0~0~0~0~0 ++
-       format_word ◦ constant wzero 24 ++ format_enum EtherTypeCodes ◦ EthType ++ empty_Format) s env t ->
-      bs = true) /\ ((format_enum EtherTypeCodes ◦ EthType ++ empty_Format) s env t -> bs = false)).
+       format_word ◦ constant wzero 24 ++ format_enum EtherTypeCodes ◦ EthType ++ empty_Format) s env
+        (mappend (fst t) t', env') -> bs = true) /\
+     ((format_enum EtherTypeCodes ◦ EthType ++ empty_Format) s env (mappend (fst t) t', env') -> bs = false)).
   Proof.
-  Admitted.
-
-  (*Lemma v1042_OKT
-    : forall (data : EthernetHeader) (bin : ByteString) (env xenv : CacheFormat) (ext : ByteString),
-      ((   format_nat 16 ◦ constant packet_len
-        ++ format_word ◦ constant WO~0~1~0~1~0~1~0~1
-        ++ format_word ◦ constant WO~0~1~0~1~0~1~0~1
-        ++ format_word ◦ constant WO~1~1~0~0~0~0~0~0
-        ++ format_word ◦ constant (wzero 24)
-        ++ format_enum EtherTypeCodes ◦ EthType
-        ++ empty_Format ) data env) ↝ (bin, xenv)
-      -> v1042_test (mappend bin ext) = true.
-  Proof.
-    intros.
-    unfold sequence_Format, compose at 1, Bind2 in H;
-      computes_to_inv; destruct v; destruct v0.
-        injections.
-    pose proof mappend_assoc as H'''; simpl in H'''; rewrite <- H'''.
-    unfold v1042_test.
-    pose proof (monoid_get_encode_word' 16 (natToWord 16 packet_len)) as H''''.
-    apply EquivFormat_Projection_Format in H.
-    unfold format_nat, format_word in H; computes_to_inv.
-    apply (f_equal fst) in H; simpl in H.
-    rewrite <- H.
-    simpl mappend in *.
-    rewrite H''''.
-    find_if_inside; eauto.
-    destruct n.
-    eapply natToWord_wlt; eauto; try reflexivity.
-    etransitivity.
-    unfold BinNat.N.lt; rewrite <- Nnat.Nat2N.inj_compare.
-    eapply Compare_dec.nat_compare_lt; eassumption.
-    reflexivity.
+    split; intros.
+    - econstructor; intros.
+      + unfold format_unused_word, Compose_Format in H1.
+        rewrite unfold_computes in H1; destruct_ex; split_and.
+        eapply @Word_decode_correct with (P := P) in H2; eauto.
+        destruct_ex; split_and.
+        rewrite H2; simpl; subst.
+        destruct (wlt_dec x0 (natToWord 16 1501)); simpl.
+        * eexists _, _; intuition eauto.
+          apply unfold_computes; intuition eauto.
+          unfold sequence_Format, Projection_Format, empty_Format,
+          Compose_Format, ComposeOpt.compose, Bind2 in H1.
+          apply unfold_computes in H1; computes_to_inv.
+          rewrite unfold_computes in H1; destruct_ex; split_and;
+            injections; destruct v; subst.
+          pose proof mempty_right as H'; simpl in H'; rewrite H' in H11;
+            subst; clear H'.
+          simpl in H11; subst.
+          eapply @Enum_decode_correct with (P := P) in H8; try eassumption.
+          eapply @Word_decode_correct with (P := P) in H6; try eassumption.
+          destruct_ex; split_and.
+          unfold decode_enum in H8.
+          instantiate (1 := mempty) in H8.
+          pose proof mempty_right as H'; simpl in H'; rewrite H' in H8;
+            subst; clear H'.
+          rewrite H12 in H8; simpl in H8.
+          destruct (word_indexed x3 EtherTypeCodes) eqn: ?; try discriminate;
+            simpl in H8.
+          injections.
+          unfold word_indexed in Heqo; simpl in Heqo.
+          repeat match type of Heqo with
+                   context[weqb ?a ?b] =>
+                   let H := fresh in destruct (weqb a b) eqn : H;
+                                       try apply weqb_sound in H; subst
+                 end.
+          injections.
+          Local Transparent natToWord.
+          unfold natToWord in w; compute in w; discriminate.
+          unfold natToWord in w; compute in w; discriminate.
+          unfold natToWord in w; compute in w; discriminate.
+          unfold natToWord in w; compute in w; discriminate.
+          discriminate.
+          Discharge_NoDupVector.
+        * eexists _, _; intuition eauto.
+          apply unfold_computes; intuition eauto.
+          unfold sequence_Format at 1, Projection_Format, empty_Format,
+          Compose_Format, ComposeOpt.compose, Bind2 in H1.
+          apply unfold_computes in H1; computes_to_inv.
+          rewrite unfold_computes in H1; destruct_ex; split_and;
+            injections; destruct v; subst.
+          clear H1'.
+          simpl in H11.
+          eapply @Nat_decode_correct with (P := P) in H8; try eassumption.
+          eapply @Word_decode_correct with (P := P) in H6; try eassumption.
+          simpl in H8; rewrite H11 in H8.
+          destruct_ex; split_and.
+          unfold decode_nat in H8.
+          rewrite H13 in H8; simpl in H8.
+          injections; subst.
+          destruct n.
+          unfold wlt.
+          rewrite !wordToN_nat, wordToNat_natToWord_idempotent.
+          eapply Nomega.Nlt_in.
+          rewrite !Nnat.Nat2N.id.
+          eauto.
+          reflexivity.
+          etransitivity; try eassumption.
+          rewrite <- Nnat.Nat2N.id.
+          rewrite <- (Nnat.Nat2N.id 1501).
+          apply Nomega.Nlt_out.
+          reflexivity.
+      + destruct (decode_word t env') as [ [ [? ?] ?] | ] eqn: ? ; simpl in H1;
+          try discriminate.
+        generalize Heqo; intros.
+        eapply @Word_decode_correct with (P := P) in Heqo; try eassumption.
+        destruct (wlt_dec w (natToWord 16 1501)) eqn: ?; simpl in H1;
+          try discriminate; injections; intuition eauto;
+            destruct_ex; split_and;
+              subst; eexists _, _; intuition eauto.
+        * apply unfold_computes; intros; intros; split; eauto.
+          split; simpl; intros; eauto.
+          unfold sequence_Format, Projection_Format, Compose_Format,
+          ComposeOpt.compose, Bind2 in H2.
+          apply unfold_computes in H2; computes_to_inv; subst.
+          rewrite unfold_computes in H2; destruct_ex; split_and; subst.
+          destruct v; destruct v2; injections.
+          eapply @Word_decode_correct with (P := P) in H3; try eassumption.
+          eapply @Enum_decode_correct with (P := P) in H5; try eassumption.
+          destruct_ex; split_and.
+          unfold decode_enum in H10.
+          rewrite <- H7 in H5.
+          rewrite H5 in H10; simpl in H10.
+          unfold word_indexed in H10; simpl in H10.
+          repeat match type of H10 with
+                   context[weqb ?a ?b] =>
+                   let H := fresh in destruct (weqb a b) eqn : H;
+                                       try apply weqb_sound in H; subst
+                 end; simpl in H10; try discriminate.
+          Discharge_NoDupVector.
+        * apply unfold_computes; intros; intros; split; eauto.
+          split; simpl; intros; eauto.
+          unfold sequence_Format at 1, Projection_Format, Compose_Format,
+          ComposeOpt.compose, Bind2 in H2.
+          apply unfold_computes in H2; computes_to_inv; subst.
+          clear H2'.
+          rewrite unfold_computes in H2; destruct_ex; split_and; subst.
+          destruct v; destruct v2; injections.
+          eapply @Word_decode_correct with (P := P) in H3; try eassumption.
+          eapply @Nat_decode_correct with (P := P) in H5; try eassumption.
+          destruct_ex; split_and.
+          unfold decode_nat in H10.
+          rewrite <- H7 in H5.
+          rewrite H5 in H10; simpl in H10; injections.
+          destruct n.
+          unfold wlt.
+          rewrite !wordToN_nat, wordToNat_natToWord_idempotent.
+          eapply Nomega.Nlt_in.
+          rewrite !Nnat.Nat2N.id.
+          eauto.
+          reflexivity.
+          etransitivity; try eassumption.
+          rewrite <- Nnat.Nat2N.id.
+          rewrite <- (Nnat.Nat2N.id 1501).
+          apply Nomega.Nlt_out.
+          reflexivity.
+    - unfold composeIf, Union_Format in H; rewrite unfold_computes in H.
+      destruct_ex; revert H; pattern x;
+        apply IterateBoundedIndex.Iterate_Ensemble_BoundedIndex_equiv; simpl;
+          econstructor; [intros | econstructor; intros; eauto].
+      Opaque natToWord.
+      + unfold Vector.nth in H; simpl in H.
+        unfold sequence_Format at 1 in H.
+        unfold Projection_Format, empty_Format,
+        Compose_Format, ComposeOpt.compose, Bind2 in H.
+        computes_to_inv.
+        rewrite unfold_computes in H; destruct_ex; split_and;
+          subst; eauto.
+        unfold format_nat, format_word in H0; computes_to_inv; subst.
+        injections; eexists _, _, _; intuition eauto.
+        unfold format_unused_word, Compose_Format.
+        apply unfold_computes; eexists _; intuition eauto;
+          try computes_to_econstructor.
+        apply unfold_computes; eauto.
+      + unfold Vector.nth in H; simpl in H.
+        unfold sequence_Format at 1 in H.
+        unfold Projection_Format, empty_Format,
+        Compose_Format, ComposeOpt.compose, Bind2 in H.
+        computes_to_inv.
+        rewrite unfold_computes in H; destruct_ex; split_and;
+          subst; eauto.
+        unfold format_enum, format_word in H0; computes_to_inv; subst.
+        injections; eexists _, _, _; intuition eauto.
+        unfold format_unused_word, Compose_Format.
+        apply unfold_computes; eexists _; intuition eauto;
+          try computes_to_econstructor.
+        apply unfold_computes; eauto.
+        Grab Existential Variables.
+        eauto.
+        eauto.
   Qed.
-
-  (*Hint Extern 4 => eapply v1042_OKT : bin_split_hints. *)
-
-    Lemma v1042_OKE
-    : forall (data : EthernetHeader) (bin : ByteString) (env xenv : CacheFormat) (ext : ByteString),
-      (   format_enum EtherTypeCodes ◦ EthType
-       ++ empty_Format) data env ↝ (bin, xenv)
-      -> v1042_test (mappend bin ext) = false.
-  Proof.
-    intros.
-    apply NormalizeFormats.EquivFormat_Projection_Format_Empty_Format in H.
-    apply EquivFormat_Projection_Format in H.
-    unfold compose, Bind2, format_enum, format_word in H; computes_to_inv; subst.
-    injections.
-    (*pose proof (f_equal fst H'') as H'; unfold fst in H'; rewrite <- H'. *)
-    unfold v1042_test.
-    pose monoid_get_encode_word' as H'''; rewrite H'''; find_if_inside; eauto.
-    revert w; clear.
-    match goal with
-      |- context [Vector.nth (m := ?n) ?w ?idx] => remember idx; clear
-    end.
-    eapply forall_Vector_P; repeat econstructor;
-      unfold wlt; compute; intros; discriminate.
-  Qed. *)
-
-  (*Hint Extern 4 => eapply v1042_OKE : bin_split_hints. *)
 
   Lemma valid_packet_len_OK_good_Len
     : lt packet_len (pow2 16).
@@ -177,154 +277,18 @@ Section EthernetPacketDecoder.
 
   Hint Extern 4 => eapply valid_packet_len_OK_good_Len : data_inv_hints.
 
-  (*Definition aligned_v1042_test
-        {sz : nat}
-        (v : t Core.char sz)
-        (idx : nat)
-    : bool :=
-    match nth_opt v idx, nth_opt v (S idx) with
-    | Some w1, Some w2 =>
-      if wlt_dec (combine w2 w1) (natToWord 16 1501) then true else false
-    | _, _ => false
-    end.
-
-  Lemma aligned_v1042_test_OK_1 {sz}
-    : forall (v : t Core.char sz),
-      v1042_test (build_aligned_ByteString v) =
-      aligned_v1042_test v 0.
-  Proof.
-    destruct v.
-    reflexivity.
-    destruct v.
-    reflexivity.
-    unfold v1042_test.
-    replace (monoid_get_word 16 (build_aligned_ByteString (h :: h0 :: v)))
-      with
-        (Some (combine h0 h)).
-    reflexivity.
-    replace (build_aligned_ByteString (h :: h0 :: v))
-      with (mappend (build_aligned_ByteString (h :: h0 :: Vector.nil _)) (build_aligned_ByteString v)).
-    rewrite <- (monoid_get_encode_word' _ (combine h0 h) (build_aligned_ByteString v)).
-    f_equal.
-    f_equal.
-    simpl.
-    unfold Core.char in *.
-    shatter_word h.
-    shatter_word h0.
-    simpl.
-    rewrite build_aligned_ByteString_cons; simpl.
-    unfold ByteString_enqueue_ByteString; simpl.
-    unfold ByteString_enqueue_char.
-    simpl.
-    repeat f_equal.
-    unfold build_aligned_ByteString; simpl.
-    erewrite (ByteString_enqueue_simpl x6); simpl.
-    erewrite (ByteString_enqueue_simpl x5); simpl.
-    erewrite (ByteString_enqueue_simpl x4); simpl.
-    erewrite (ByteString_enqueue_simpl x3); simpl.
-    erewrite (ByteString_enqueue_simpl x2); simpl.
-    erewrite (ByteString_enqueue_simpl x1); simpl.
-    erewrite (ByteString_enqueue_simpl x0); simpl.
-    unfold ByteString_enqueue; simpl.
-    f_equal.
-    eapply Core.le_uniqueness_proof.
-    simpl.
-    rewrite <- build_aligned_ByteString_append.
-    reflexivity.
-    Grab Existential Variables.
-    simpl; omega.
-    simpl; omega.
-    simpl; omega.
-    simpl; omega.
-    simpl; omega.
-    simpl; omega.
-    simpl; omega.
-  Qed.
-
-  Lemma aligned_v1042_test_OK_2 {sz}
-    : forall (v : ByteBuffer.t (S sz)) (idx : nat),
-      aligned_v1042_test v (S idx) = aligned_v1042_test (Vector.tl v) idx.
-  Proof.
-    intros; pattern sz, v; eapply Vector.caseS; higher_order_reflexivity.
-  Qed.
-
-  Hint Extern 4 => eapply aligned_v1042_test_OK_1.
-  Hint Extern 4 => eapply aligned_v1042_test_OK_2. *)
-
-  Create HintDb bin_split_hints.
-
-Ltac apply_combinator_rule apply_rules ::=
-  apply_combinator_rule'
-    continue_on_fail
-
-    halt_on_fail_1
-    halt_on_fail
-
-    continue_on_fail_2
-    continue_on_fail_1
-    halt_on_fail
-
-    apply_rules.
+  Ltac apply_new_combinator_rule ::=
+    match goal with
+    | H : cache_inv_Property ?mnd _
+      |- context[CorrectRefinedDecoder] =>
+      eapply (@derive_distinguishing_word _ _ _ H); eauto
+  end.
 
   Definition EthernetHeader_decoder
     : CorrectAlignedDecoderFor ethernet_Header_OK EthernetHeader_Format.
   Proof.
     synthesize_aligned_decoder.
-    eapply composeIf_format_correct'; intros.
-    apply H; intros.
-    apply_rules.
-    apply_rules.
-    eapply derive_distinguishing_word.
-    exact H2.
-    synthesize_cache_invariant.
-    unfold v1042_test.
-    cbv beta; unfold decode_nat, sequence_Decode.
-    optimize_decoder_impl.
-    cbv beta; simpl; align_decoders.
-  Admitted.
-  (*cbv beta; simpl; align_decoders.
-    eapply @AlignedDecodeBind2CharM
-    ; intros; eauto.
-
-first
-  [ eapply @AlignedDecodeNatM; intros
-  | eapply @AlignedDecodeByteBufferM; intros; eauto
-  | eapply @AlignedDecodeBind2CharM; intros; eauto
-  | eapply @AlignedDecodeBindCharM; intros; eauto
-  | eapply @AlignedDecodeBind3CharM; intros; eauto
-  | eapply @AlignedDecodeBind4CharM; intros; eauto
-  | eapply @AlignedDecodeBindEnum; intros; eauto
-  | let H' := fresh in
-    pose proof (fun C D => @AlignedDecodeBindEnumM _ _ C D 2) as H'; simpl in H'; eapply H'; eauto; intros
-  | eapply @AlignedDecodeBindUnused2CharM; simpl; eauto; eapply DecodeMEquivAlignedDecodeM_trans;
-     [  | intros; reflexivity |  ]
-  | eapply @AlignedDecodeBindUnusedCharM; simpl; eauto; eapply DecodeMEquivAlignedDecodeM_trans;
-     [  | intros; reflexivity |  ]
-  | eapply @AlignedDecodeListM; intros; eauto
-  | eapply @AlignedDecodeCharM; intros; eauto
-  | eapply (fun H H' => AlignedDecodeNCharM H H'); eauto; simpl; intros
-  | eapply (fun H H' => AlignedDecodeNCharM H H'); eauto; simpl; intros
-  | eapply (AlignedDecodeNUnusedCharM _ _); eauto; simpl; intros
-  | eapply @AlignedDecode_shift_if_Sumb
-  | eapply @AlignedDecode_shift_if_bool
-  | eapply @Return_DecodeMEquivAlignedDecodeM
-  | eapply @AlignedDecode_Sumb
-  | eapply AlignedDecode_ifopt; intros
-  | let H := fresh in
-    pose proof @AlignedDecode_if_Sumb_dep as H; eapply H; clear H; [ solve [ eauto ] | solve [ eauto ] |  |  ]
-  | eapply @AlignedDecode_ifb
-  | eapply @AlignedDecode_ifb_both
-  | eapply @AlignedDecode_ifb_dep; [ solve [ eauto ] | solve [ eauto ] |  |  ]
-  | eapply @AlignedDecodeBindOption; intros; eauto
-  | eapply @AlignedDecode_Throw
-  | intros; higher_order_reflexivity
-  | eapply @AlignedDecode_CollapseEnumWord
-  | eapply @AlignedDecode_CollapseWord'; eauto
-     using decode_word_eq_decode_unused_word, decode_word_eq_decode_bool, decode_word_eq_decode_nat,
-       decode_word_eq_decode_word ].
-
-
-  Defined. *)
+  Defined.
 
   (* Step Four: Extract the decoder function, and have /it/ start decoding
      at the start of the provided ByteString [v]. *)
